lib/core/Pulse.Lib.Loc.fst
@@ -1,0 +1,12 @@
+module Pulse.Lib.Loc
+
+[@@erased]
+noeq type loc_id = {
+  process: nat;
+  thread: nat;
+}
+
+let process_of l = { l with thread = 0 }
+let process_of_idem l = ()
+
+let dummy_loc = { process = 0; thread = 0 }
