lib/pulse/lib/Pulse.Lib.GhostReference.fst
@@ -20,6 +20,7 @@ open Pulse.Lib.Core
 open Pulse.Main
 open FStar.PCM
 open Pulse.Lib.PCM.Fraction
+open Pulse.Lib.SendSync
 module GR = Pulse.Lib.GhostPCMReference
 module T = FStar.Tactics
 let ref a = GR.ghost_pcm_ref #_ (pcm_frac #a)
@@ -29,6 +30,7 @@ let null #a = GR.null_core_ghost_pcm_ref
 let pts_to (#a:Type) (r:ref a) (#[T.exact (`1.0R)] p:perm) (n:a)
 = GR.pts_to r (Some (n, p)) ** pure (perm_ok p)
 
+let pts_to_placeless r p n = Tactics.Typeclasses.solve
 let pts_to_timeless _ _ _ = ()
 
 
