lib/pulse/lib/Pulse.Lib.Inv.fsti
@@ -1,0 +1,80 @@
+module Pulse.Lib.Inv
+#lang-pulse
+open Pulse.Lib.Core
+open Pulse.Lib.SendSync
+open Pulse.Class.Duplicable
+open PulseCore.Observability
+
+val inv (i: iname) (p: slprop) : slprop
+
+ghost fn move i p l1 l2
+    (fwd: unit -> stt_ghost unit emp_inames (on l1 p) (fun _ -> on l2 p))
+    (bwd: unit -> stt_ghost unit emp_inames (on l2 p) (fun _ -> on l1 p))
+  requires on l1 (inv i p)
+  ensures on l2 (inv i p)
+
+instance val is_send_across_inv #b #g i p {| is_send_across #b g p |} : is_send_across g (inv i p)
+instance placeless_inv i p {| inst: placeless p |} : placeless (inv i p) = is_send_across_inv i p #inst
+instance is_send_inv i p {| inst: is_send p |} : is_send (inv i p) = is_send_across_inv i p #inst
+instance val duplicable_inv i p : duplicable (inv i p)
+
+ghost fn dup_inv (i:iname) (p:slprop)
+  preserves inv i p
+  ensures inv i p
+{
+  dup (inv i p) ()
+}
+
+ghost fn fresh_invariant
+    (ctx: inames { Pulse.Lib.GhostSet.is_finite ctx })
+    (p: slprop)
+  requires p
+  returns i: iname
+  ensures inv i p
+  ensures pure (~(Pulse.Lib.GhostSet.mem i ctx))
+
+ghost fn new_invariant (p: slprop)
+  requires p
+  returns i: iname
+  ensures inv i p
+
+inline_for_extraction noextract
+unobservable fn with_inv_unobs u#a (a: Type u#a)
+    is (i: iname { not (mem_inv is i) }) (p: slprop) pre (post: a->slprop)
+    (k: unit -> stt_atomic a #Neutral is (pre ** p) (fun x -> post x ** p))
+  opens add_inv is i
+  preserves inv i p
+  requires later_credit 1
+  requires pre
+  returns x:a
+  ensures post x
+
+ghost fn with_invariants_g u#a (a: Type u#a)
+    is (i: iname { not (mem_inv is i) }) (p: slprop) pre (post: a->slprop)
+    (k: unit -> stt_ghost a is (pre ** p) (fun x -> post x ** p))
+  opens add_inv is i
+  preserves inv i p
+  requires later_credit 1
+  requires pre
+  returns x:a
+  ensures post x
+
+inline_for_extraction noextract
+atomic fn with_invariants_a u#a (a: Type u#a)
+    is (i: iname { not (mem_inv is i) }) (p: slprop) pre (post: a->slprop)
+    (k: unit -> stt_atomic a #Observable is (pre ** p) (fun x -> post x ** p))
+  opens add_inv is i
+  preserves inv i p
+  requires later_credit 1
+  requires pre
+  returns x:a
+  ensures post x
+
+inline_for_extraction noextract
+fn with_invariants u#a (a: Type u#a)
+    is (i: iname { not (mem_inv is i) }) (p: slprop) pre (post: a->slprop)
+    (k: unit -> stt_atomic a #Observable is (pre ** p) (fun x -> post x ** p))
+  preserves inv i p
+  requires pre
+  returns x:a
+  ensures post x
