share/pulse/examples/parallel/ParallelFor.fst
@@ -23,6 +23,7 @@ open Pulse.Lib.Task
 open FStar.Real
 open Pulse.Lib.Pledge
 open Pulse.Lib.OnRange
+open Pulse.Lib.SendSync
 
 module P = Pulse.Lib.Pledge
 module R = Pulse.Lib.Reference
@@ -227,8 +228,8 @@ fn rec redeem_range
 
 fn
 parallel_for
-  (pre : (nat -> slprop))
-  (post : (nat -> slprop))
+  (pre : (nat -> slprop)) {| (x:nat -> is_send (pre x)) |}
+  (post : (nat -> slprop)) {| (x:nat -> is_send (post x)) |}
   (f : (i:nat -> stt unit (pre i) (fun () -> (post i))))
   (n : pos)
   requires on_range pre 0 n
@@ -280,8 +281,8 @@ spawning sequentially. *)
 
 fn
 parallel_for_alt
-  (pre : (nat -> slprop))
-  (post : (nat -> slprop))
+  (pre : (nat -> slprop)) {| (x:nat -> is_send (pre x)) |}
+  (post : (nat -> slprop)) {| (x:nat -> is_send (post x)) |}
   (f : (i:nat -> stt unit (pre i) (fun () -> (post i))))
   (n : pos)
   requires on_range pre 0 n
@@ -378,8 +379,8 @@ fn rec funfold
 
 fn
 parallel_for_wsr
-  (pre : (nat -> slprop))
-  (post : (nat -> slprop))
+  (pre : (nat -> slprop)) {| (x:nat -> is_send (pre x)) |}
+  (post : (nat -> slprop)) {| (x:nat -> is_send (post x)) |}
   (full_pre : (nat -> slprop))
   (full_post : (nat -> slprop))
   (f : (i:nat -> stt unit (pre i) (fun () -> post i)))
@@ -407,8 +408,8 @@ val frame_stt_left
 fn rec h_for_task
   (p:pool)
   (e:perm)
-  (pre : (nat -> slprop))
-  (post : (nat -> slprop))
+  (pre : (nat -> slprop)) {| (x:nat -> is_send (pre x)) |}
+  (post : (nat -> slprop)) {| (x:nat -> is_send (post x)) |}
   (f : (i:nat -> stt unit (pre i) (fun () -> post i)))
   (lo hi : nat)
   (_:unit)
@@ -421,7 +422,7 @@ fn rec h_for_task
     for_loop pre post emp
              (fun i -> frame_stt_left emp (f i)) lo hi;
 
-    return_pledge (pool_done p) (on_range post lo hi)
+    return_pledge (pool_done p) (on_range post lo hi) #_
   } else {
     let mid = (hi+lo)/2;
     assert (pure (lo <= mid /\ mid <= hi));
@@ -482,8 +483,8 @@ val wait_pool
 
 fn
 parallel_for_hier
-  (pre : (nat -> slprop))
-  (post : (nat -> slprop))
+  (pre : (nat -> slprop)) {| (x:nat -> is_send (pre x)) |}
+  (post : (nat -> slprop)) {| (x:nat -> is_send (post x)) |}
   (f : (i:nat -> stt unit (pre i) (fun () -> (post i))))
   (n : pos)
   requires on_range pre 0 n
